proof/refine/AARCH64/Arch_R.thy
@@ -1774,12 +1774,14 @@ lemma assoc_invs':
   apply (rule conjI)
    apply (clarsimp simp: typ_at_to_obj_at_arches obj_at'_def)
   apply (rule conjI)
+   apply (clarsimp simp: valid_vcpu'_def)
+  apply (rule conjI)
    apply (clarsimp simp: typ_at_tcb' obj_at'_def)
    apply (rule_tac rfs'="state_hyp_refs_of' s" in delta_sym_refs, assumption)
     supply fun_upd_apply[simp]
     apply (clarsimp simp: hyp_live'_def arch_live'_def)
     apply (clarsimp split: if_split_asm)
-   apply (clarsimp simp: state_hyp_refs_of'_def obj_at'_def projectKOs tcb_vcpu_refs'_def
+   apply (clarsimp simp: state_hyp_refs_of'_def obj_at'_def tcb_vcpu_refs'_def
                   split: option.splits if_split_asm)
   apply (clarsimp simp: hyp_live'_def arch_live'_def)
   done
