proof/refine/AARCH64/Finalise_R.thy
@@ -2611,7 +2611,7 @@ lemma dissoc_invs':
                     state_refs_of'_vcpu_empty state_hyp_refs_of'_vcpu_absorb valid_arch_tcb'_def
         | clarsimp simp: live'_def hyp_live'_def arch_live'_def)+
   supply fun_upd_apply[simp]
-  apply (clarsimp simp: state_hyp_refs_of'_def obj_at'_def tcb_vcpu_refs'_def
+  apply (clarsimp simp: state_hyp_refs_of'_def obj_at'_def tcb_vcpu_refs'_def valid_vcpu'_def
                   split: option.splits if_split_asm)
   apply safe
    apply (rule_tac rfs'="state_hyp_refs_of' s" in delta_sym_refs)
