proof/refine/AARCH64/KHeap_R.thy
@@ -1113,18 +1113,19 @@ lemma typ_at'_valid_obj'_lift:
   notes [wp] = hoare_vcg_all_lift hoare_vcg_imp_lift hoare_vcg_const_Ball_lift typ_at_lifts [OF P]
   shows      "\<lbrace>\<lambda>s. valid_obj' obj s\<rbrace> f \<lbrace>\<lambda>rv s. valid_obj' obj s\<rbrace>"
   apply (cases obj; simp add: valid_obj'_def hoare_TrueI)
-     apply (rename_tac endpoint)
-     apply (case_tac endpoint; simp add: valid_ep'_def, wp)
-    apply (rename_tac notification)
-    apply (case_tac "ntfnObj notification";
+      apply (rename_tac endpoint)
+      apply (case_tac endpoint; simp add: valid_ep'_def, wp)
+     apply (rename_tac notification)
+     apply (case_tac "ntfnObj notification";
             simp add: valid_ntfn'_def valid_bound_tcb'_def split: option.splits,
             (wpsimp|rule conjI)+)
-   apply (rename_tac tcb)
-   apply (case_tac "tcbState tcb";
-          simp add: valid_tcb'_def valid_tcb_state'_def split_def valid_bound_ntfn'_def
-             split: option.splits,
-          wpsimp)
-  apply (wpsimp simp: valid_cte'_def)
+    apply (rename_tac tcb)
+    apply (case_tac "tcbState tcb";
+           simp add: valid_tcb'_def valid_tcb_state'_def split_def valid_bound_ntfn'_def
+              split: option.splits,
+           wpsimp)
+   apply (wpsimp simp: valid_cte'_def)
+  apply wp
   done
 
 lemmas setObject_valid_obj = typ_at'_valid_obj'_lift [OF setObject_typ_at']
